

which is very much like recurrence (4.19). Indeed, this new recurrence has the same solution: $S(m) = O(m \lg m)$. Changing back from $S(m)$ to $T(n)$, we obtain $T(n) = T(2^m) = S(m) = O(m \lg m) = O(\lg n \lg \lg n)$.

Exercises

4.3-1

Show that the solution of $T(n) = T(n-1) + n$ is $O(n^2)$.

4.3-2

Show that the solution of $T(n) = T(\lceil n/2 \rceil) + 1$ is $O(\lg n)$.

4.3-3

We saw that the solution of $T(n) = 2T(\lfloor n/2 \rfloor) + n$ is $O(n \lg n)$. Show that the solution of this recurrence is also $\Omega(n \lg n)$. Conclude that the solution is $\Theta(n \lg n)$.

4.3-4

Show that by making a different inductive hypothesis, we can overcome the difficulty with the boundary condition $T(1) = 1$ for recurrence (4.19) without adjusting the boundary conditions for the inductive proof.

4.3-5

Show that $\Theta(n \lg n)$ is the solution to the “exact” recurrence (4.3) for merge sort.

4.3-6

Show that the solution to $T(n) = 2T(\lfloor n/2 \rfloor + 17) + n$ is $O(n \lg n)$.

4.3-7

Using the master method in Section 4.5, you can show that the solution to the recurrence $T(n) = 4T(n/3) + n$ is $T(n) = \Theta(n^{\log_3 4})$. Show that a substitution proof with the assumption $T(n) \leq cn^{\log_3 4}$ fails. Then show how to subtract off a lower-order term to make a substitution proof work.

4.3-8

Using the master method in Section 4.5, you can show that the solution to the recurrence $T(n) = 4T(n/2) + n^2$ is $T(n) = \Theta(n^2)$. Show that a substitution proof with the assumption $T(n) \leq cn^2$ fails. Then show how to subtract off a lower-order term to make a substitution proof work.

4.3-1

Show that the solution of $T(n) = T(n-1) + n$ is $O(n^2)$.

$$T(n) = O(n^2)$$

$$T(n) \leq cn^2$$

$$T(1) + n - n^2 \leq cn^2$$

→ Constante positiva

Supondo $T(1) = 1 : T(1) \leq cn^2$

$$T(1) \leq c$$

$$1 \leq c \checkmark$$

$$T(n) = T(n-1) + n = T(n-2) + n + n = T(n-2) + 2n$$

$$T(n-1) = T(n-2) + n$$

$$T(n) = T(n-k) + kn$$

$$T(n) = T(n-n+1) + (1-n)n$$

$$T(n) = T(1) + n - n^2$$

$$n - k = 1$$

$$k = 1 - n$$

$$c(n^2 - 2n + 1) + n$$

$$T(n) \leq cn^2$$

$$T(n-1) \leq c(n-1)^2$$

$$T(n) \leq c(n-1)^2 + n$$

$$T(n) \leq cn^2 - 2cn + c + n$$

$$cn^2 - 2cn + c + n \leq cn^2$$

$$-2cn + c + n \leq 0 \quad c = 1$$

$$n(-2c+1) + c \leq 0 \quad \checkmark \quad n \geq 1$$